theories/Prelude/PreludeInit.v
@@ -443,6 +443,9 @@ Module PreludeInit_main.
 
   End ImplFor_ensemble.
 
+  Global Arguments isSameSetAs {A} (lhs) (rhs) : simpl never.
+  Global Arguments isSubsetOf {A} (lhs) (rhs) : simpl never.
+
   Section ImplFor_pair.
 
   Variable fsts : Hask.t.
@@ -863,24 +866,3 @@ Module E.
   .
 
 End E.
-
-Module MathNotations.
-
-  Global Declare Scope math_scope.
-  Global Declare Custom Entry math_viewer.
-
-  Global Bind Scope math_scope with not Funclass eqProp leProp and or impl iff.
-
-  Global Notation " '$' e '$' " := e (e custom math_viewer at level 11, at level 0, no associativity) : math_scope.
-  Global Notation " e " := e (in custom math_viewer at level 0, e ident).
-  Global Notation " '[|' e '|]' " := e (in custom math_viewer, e constr).
-  Global Notation " '(' e ')' " := e (in custom math_viewer, e at level 11).
-  Global Notation " '~' e " := (not e) (in custom math_viewer at level 7, right associativity).
-  Global Notation " A '->' B " := (A -> B) (in custom math_viewer at level 10, right associativity).
-  Global Infix " '==' " := eqProp (in custom math_viewer at level 7, no associativity).
-  Global Infix " '=<' " := leProp (in custom math_viewer at level 7, no associativity).
-  Global Infix " '/\' " := and (in custom math_viewer at level 8, right associativity).
-  Global Infix " '\/' " := or (in custom math_viewer at level 9, right associativity).
-  Global Infix " '<->' " := iff (in custom math_viewer at level 10, no associativity).
-
-End MathNotations.
